my hands are typing words

Bytestring/Decode.lean
@@ -1,33 +1,121 @@
 import Bytestring.ByteArray
 
-section decode
+/-! # `List` lemmas -/
 
-inductive FirstByte where
-  | invalid : FirstByte
-  | done : FirstByte
-  | oneMore : FirstByte
-  | twoMore : FirstByte
-  | threeMore : FirstByte
+theorem List.eq_getElem_of_length_eq_one : (l : List α) → (hl : l.length = 1) → l = [l[0]]
+  | [_], _ => rfl
 
-inductive LaterByte where
-  | invalid : LaterByte
-  | valid : (b : UInt8) → b < 0x40 → LaterByte
+theorem List.eq_getElem_of_length_eq_two : (l : List α) → (hl : l.length = 2) → l = [l[0], l[1]]
+  | [_, _], _ => rfl
 
-instance : Trans (· ≤ · : UInt8 → UInt8 → Prop) (· < · : UInt8 → UInt8 → Prop) (· < ·) where
-  trans := UInt8.lt_of_le_of_lt
+theorem List.eq_getElem_of_length_eq_three : (l : List α) → (hl : l.length = 3) → l = [l[0], l[1], l[2]]
+  | [_, _, _], _ => rfl
 
--- abbrev UInt8.maxValue : UInt8 := 0xFF
+theorem List.eq_getElem_of_length_eq_four : (l : List α) → (hl : l.length = 4) → l = [l[0], l[1], l[2], l[3]  ]
+  | [_, _, _, _], _ => rfl
 
--- @[simp] theorem UInt8.toBitVec_maxValue : UInt8.maxValue.toBitVec = BitVec.allOnes _ := rfl
-
--- @[simp] theorem UInt8.and_maxValue {b : UInt8} : b &&& UInt8.maxValue = b :=
---   UInt8.eq_of_toBitVec_eq (by rw [UInt8.toBitVec_and, toBitVec_maxValue, BitVec.and_allOnes])
+/-! # `BitVec` lemmas -/
 
 theorem BitVec.and_or_distrib_left {a b c : BitVec w} : a &&& (b ||| c) = (a &&& b) ||| (a &&& c) :=
   BitVec.eq_of_getElem_eq (by simp [Bool.and_or_distrib_left])
 
 theorem BitVec.and_or_distrib_right {a b c : BitVec w} : (a ||| b) &&& c = (a &&& c) ||| (b &&& c) :=
   BitVec.eq_of_getElem_eq (by simp [Bool.and_or_distrib_right])
+
+theorem BitVec.extractLsb'_setWidth_of_le {b : BitVec w} {start len w' : Nat} (h : start + len ≤ w') :
+    (b.setWidth w').extractLsb' start len = b.extractLsb' start len := by
+  ext i h_i
+  simp
+  omega
+
+theorem BitVec.extractLsb'_append_eq_left {a : BitVec w} {b : BitVec w'} : (a ++ b).extractLsb' w' w = a := by
+  simp [BitVec.extractLsb'_append_eq_of_le]
+
+theorem BitVec.extractLsb'_append_eq_right {a : BitVec w} {b : BitVec w'} : (a ++ b).extractLsb' 0 w' = b := by
+  simp [BitVec.extractLsb'_append_eq_of_add_le]
+
+theorem BitVec.setWidth_append_eq_right {a : BitVec w} {b : BitVec w'} : (a ++ b).setWidth w' = b := by
+  ext i hi
+  simp [getLsbD_append, hi]
+
+theorem BitVec.setWidth_setWidth_eq_self {a : BitVec w} {w' : Nat} (h : a < BitVec.twoPow w w') : (a.setWidth w').setWidth w = a := by
+  by_cases hw : w' < w
+  · simp only [toNat_eq, toNat_setWidth]
+    rw [Nat.mod_mod_of_dvd' (Nat.pow_dvd_pow _ (Nat.le_of_lt hw)), Nat.mod_eq_of_lt]
+    rwa [BitVec.lt_def, BitVec.toNat_twoPow_of_lt hw] at h
+  · rw [BitVec.lt_def, BitVec.toNat_twoPow_of_le (by omega)] at h
+    simp at h
+
+theorem BitVec.append_left_inj {s₁ s₂ : BitVec w} (t : BitVec w') : s₁ ++ t = s₂ ++ t ↔ s₁ = s₂ := by
+  refine ⟨fun h => ?_, fun h => h ▸ rfl⟩
+  ext i hi
+  simpa [getElem_append, dif_neg] using congrArg (·[i + w']'(by omega)) h
+
+theorem BitVec.append_right_inj (s : BitVec w) {t₁ t₂ : BitVec w'} : s ++ t₁ = s ++ t₂ ↔ t₁ = t₂ := by
+  refine ⟨fun h => ?_, fun h => h ▸ rfl⟩
+  ext i hi
+  simpa [getElem_append, hi] using congrArg (·[i]) h
+
+theorem BitVec.cast_extractLsb' {x : BitVec w} {start len₁ len₂ : Nat} (h : len₁ = len₂) :
+    (x.extractLsb' start len₁).cast h = x.extractLsb' start len₂ := by
+  cases h; simp
+
+theorem extractLsb'_append_extractLsb'_eq_extractLsb'_better {x : BitVec w} (h : start₂ = start₁ + len₁) :
+    ((x.extractLsb' start₂ len₂) ++ (x.extractLsb' start₁ len₁)) =
+    (x.extractLsb' start₁ (len₂ + len₁)) := by
+  rw [BitVec.extractLsb'_append_extractLsb'_eq_extractLsb' h, BitVec.cast_extractLsb']
+
+theorem BitVec.and_setWidth_allOnes (w' w : Nat) (b : BitVec (w' + w)) :
+    b &&& (BitVec.allOnes w).setWidth (w' + w) = 0#w' ++ b.setWidth w := by
+  ext i hi
+  simp only [getElem_and, getElem_setWidth, getLsbD_allOnes]
+  rw [BitVec.getElem_append]
+  split <;> simp_all
+
+theorem BitVec.setWidth_shiftRight {b : BitVec w} : (b >>> w').setWidth w'' = b.extractLsb' w' w'' := by
+  ext i hi
+  simp
+
+theorem BitVec.setWidth_extractLsb'_of_le {c : BitVec w} (h : len₁ ≤ len₂) :
+    (c.extractLsb' start len₂).setWidth len₁ = c.extractLsb' start len₁ := by
+  ext i hi
+  simp [show i < len₂ by omega]
+
+theorem BitVec.length_pos_of_lt {b b' : BitVec w} (h : b < b') : 0 < w :=
+  length_pos_of_ne (BitVec.ne_of_lt h)
+
+theorem BitVec.not_lt_iff {b : BitVec w} : ~~~b < b ↔ 0 < w ∧ b.msb = true := by
+  refine ⟨fun h => ?_, fun ⟨hw, hb⟩ => ?_⟩
+  · have := length_pos_of_lt h
+    exact ⟨this, by rwa [← ult_iff_lt, ult_eq_msb_of_msb_neq (by simp_all)] at h⟩
+  · rwa [← ult_iff_lt, ult_eq_msb_of_msb_neq (by simp_all)]
+
+theorem BitVec.setWidth_append_eq_shiftLeft_setWidth_or {b : BitVec w} {b' : BitVec w'} :
+    (b ++ b').setWidth w'' = (b.setWidth w'' <<< w') ||| b'.setWidth w'' := by
+  ext i hi
+  simp only [getElem_setWidth, getElem_or, getElem_shiftLeft]
+  rw [getLsbD_append]
+  split <;> simp_all
+
+theorem BitVec.setWidth_append_append_eq_shiftLeft_setWidth_or {b : BitVec w} {b' : BitVec w'} {b'' : BitVec w''} :
+    (b ++ b' ++ b'').setWidth w''' = (b.setWidth w''' <<< (w' + w'')) ||| (b'.setWidth w''' <<< w'') ||| b''.setWidth w''' := by
+  rw [BitVec.setWidth_append_eq_shiftLeft_setWidth_or,
+    BitVec.setWidth_append_eq_shiftLeft_setWidth_or,
+    BitVec.shiftLeft_or_distrib, BitVec.shiftLeft_add]
+
+theorem BitVec.setWidth_append_append_append_eq_shiftLeft_setWidth_or {b : BitVec w} {b' : BitVec w'} {b'' : BitVec w''} {b''' : BitVec w'''} :
+    (b ++ b' ++ b'' ++ b''').setWidth w'''' = (b.setWidth w'''' <<< (w' + w'' + w''')) ||| (b'.setWidth w'''' <<< (w'' + w''')) |||
+      (b''.setWidth w'''' <<< w''') ||| b'''.setWidth w'''' := by
+  simp only [BitVec.setWidth_append_eq_shiftLeft_setWidth_or, BitVec.shiftLeft_or_distrib, BitVec.shiftLeft_add]
+
+theorem BitVec.toNat_setWidth_of_le {w w' : Nat} {b : BitVec w} (h : w ≤ w') : (b.setWidth w').toNat = b.toNat := by
+  rw [BitVec.toNat_setWidth, Nat.mod_eq_of_lt]
+  exact BitVec.toNat_lt_twoPow_of_le h
+
+/-! # `UInt8` lemmas -/
+
+instance : Trans (· ≤ · : UInt8 → UInt8 → Prop) (· < · : UInt8 → UInt8 → Prop) (· < ·) where
+  trans := UInt8.lt_of_le_of_lt
 
 theorem UInt8.and_or_distrib_left {a b c : UInt8} : a &&& (b ||| c) = (a &&& b) ||| (a &&& c) :=
   UInt8.eq_of_toBitVec_eq (by simp [BitVec.and_or_distrib_left])
@@ -40,15 +128,6 @@ theorem UInt8.le_of_and_not_eq_zero {b c : UInt8} (h : b &&& ~~~c = 0) : b ≤ c
     b = b &&& (c ||| ~~~c) := by simp
     _ = b &&& c := by simp only [UInt8.and_or_distrib_left, h, UInt8.or_zero]
     _ ≤ c := and_le_right
-
-theorem BitVec.length_pos_of_lt {b b' : BitVec w} (h : b < b') : 0 < w :=
-  length_pos_of_ne (BitVec.ne_of_lt h)
-
-theorem BitVec.not_lt_iff {b : BitVec w} : ~~~b < b ↔ 0 < w ∧ b.msb = true := by
-  refine ⟨fun h => ?_, fun ⟨hw, hb⟩ => ?_⟩
-  · have := length_pos_of_lt h
-    exact ⟨this, by rwa [← ult_iff_lt, ult_eq_msb_of_msb_neq (by simp_all)] at h⟩
-  · rwa [← ult_iff_lt, ult_eq_msb_of_msb_neq (by simp_all)]
 
 theorem UInt8.not_lt_iff {b : UInt8} : ~~~b < b ↔ b.toBitVec.msb = true := by
   simp [UInt8.lt_iff_toBitVec_lt, BitVec.not_lt_iff]
@@ -66,16 +145,28 @@ theorem UInt8.lt_add_one {c : UInt8} (h : c ≠ -1) : c < c + 1 := by
   simp only [toNat_neg, UInt8.reduceToNat, Nat.add_one_sub_one, Nat.mod_succ, ne_eq] at h
   rw [UInt8.lt_iff_toNat_lt, UInt8.toNat_add]
   simp only [UInt8.reduceToNat, Nat.reducePow]
-
   rw [Nat.mod_eq_of_lt (by have := c.toNat_lt; omega)]
   omega
 
 theorem UInt8.and_lt_add_one {b c : UInt8} (h : c ≠ -1) : b &&& c < c + 1 :=
   UInt8.lt_of_le_of_lt UInt8.and_le_right (UInt8.lt_add_one h)
 
+section decode
+
+/-! # `parseFirstByte` -/
+
+/-! ## `parseFirstByte` definition -/
+
+inductive FirstByte where
+  | invalid : FirstByte
+  | done : FirstByte
+  | oneMore : FirstByte
+  | twoMore : FirstByte
+  | threeMore : FirstByte
+
 @[inline]
 def parseFirstByte (b : UInt8) : FirstByte :=
-  if b < 128 then
+  if b &&& 0x80 == 0 then
     .done
   else if b &&& 0xe0 == 0xc0 then
     .oneMore
@@ -85,12 +176,97 @@ def parseFirstByte (b : UInt8) : FirstByte :=
     .threeMore
   else .invalid
 
-theorem parseFirstByte_eq_done (b : UInt8) (hb : b ≤ 127) : parseFirstByte b = .done := by
+/-! ## `parseFirstByte` low-level API -/
+
+theorem parseFirstByte_eq_done_iff : parseFirstByte b = .done ↔ b &&& 0x80 = 0 := by
   grind [parseFirstByte]
 
-theorem parseFirstByte_eq_oneMore (b : UInt8) (hb₁ : 128 ≤ b) (hb₂ : b &&& 0xe0 = 0xc0) :
-    parseFirstByte b = .oneMore := by
-  grind [parseFirstByte]
+theorem parseFirstByte_eq_oneMore_iff : parseFirstByte b = .oneMore ↔ b &&& 0xe0 = 0xc0 := by
+  suffices b &&& 0xe0 = 0xc0 → b &&& 0x80 ≠ 0 by grind [parseFirstByte]
+  intro h
+  calc b &&& 0x80 = b &&& (0xe0 &&& 0x80) := rfl
+    _ = 0xc0 &&& 0x80 := by rw [← UInt8.and_assoc, h]
+    _ ≠ 0 := by decide
+
+theorem parseFirstByte_eq_twoMore_iff : parseFirstByte b = .twoMore ↔ b &&& 0xf0 = 0xe0 := by
+  suffices b &&& 0xf0 = 0xe0 → b &&& 0xe0 ≠ 0xc0 ∧ b &&& 0x80 ≠ 0 by grind [parseFirstByte]
+  refine fun h => ⟨?_, ?_⟩
+  · calc b &&& 0xe0 = b &&& (0xf0 &&& 0xe0) := rfl
+      _ = 0xe0 &&& 0xe0 := by rw [← UInt8.and_assoc, h]
+      _ ≠ 0xc0 := by decide
+  · calc b &&& 0x80 = b &&& (0xf0 &&& 0x80) := rfl
+      _ = 0xe0 &&& 0x80 := by rw [← UInt8.and_assoc, h]
+      _ ≠ 0 := by decide
+
+theorem parseFirstByte_eq_threeMore_iff : parseFirstByte b = .threeMore ↔ b &&& 0xf8 = 0xf0 := by
+  suffices b &&& 0xf8 = 0xf0 → b &&& 0xf0 ≠ 0xe0 ∧ b &&& 0xe0 ≠ 0xc0 ∧ b &&& 0x80 ≠ 0 by grind [parseFirstByte]
+  refine fun h => ⟨?_, ?_, ?_⟩
+  · calc b &&& 0xf0 = b &&& (0xf8 &&& 0xf0) := rfl
+      _ = 0xf0 &&& 0xf0 := by rw [← UInt8.and_assoc, h]
+      _ ≠ 0xe0 := by decide
+  · calc b &&& 0xe0 = b &&& (0xf8 &&& 0xe0) := rfl
+      _ = 0xf0 &&& 0xe0 := by rw [← UInt8.and_assoc, h]
+      _ ≠ 0xc0 := by decide
+  · calc b &&& 0x80 = b &&& (0xf8 &&& 0x80) := rfl
+      _ = 0xf0 &&& 0x80 := by rw [← UInt8.and_assoc, h]
+      _ ≠ 0 := by decide
+
+/-! ## `parseFirstByte` BitVec API -/
+
+theorem helper (w : Nat) (b : BitVec (w' + w)) (v : BitVec w') : b &&& (BitVec.allOnes w' ++ 0#w) = v ++ 0#w ↔ b.extractLsb' w w' = v := by
+  have h : b = b.extractLsb' w w' ++ b.extractLsb' 0 w := by
+    rw [extractLsb'_append_extractLsb'_eq_extractLsb'_better] <;> simp
+  conv => lhs; rw [h]
+  rw [BitVec.and_append, BitVec.and_allOnes, BitVec.and_zero, BitVec.append_left_inj]
+
+theorem helper₂ (w : Nat) (b : BitVec (w' + w)) {v : BitVec w'} (h : b.extractLsb' w w' = v) : b = v ++ b.extractLsb' 0 w := by
+  rw [← h, extractLsb'_append_extractLsb'_eq_extractLsb'_better] <;> simp
+
+/-! ### Size one -/
+
+theorem parseFirstByte_eq_done_iff_toBitVec : parseFirstByte b = .done ↔ b.toBitVec.extractLsb' 7 1 = 0#1 := by
+  simp only [parseFirstByte_eq_done_iff, ← UInt8.toBitVec_inj, UInt8.toBitVec_and,
+    UInt8.toBitVec_ofNat]
+  exact helper 7 b.toBitVec 0#1
+
+theorem toBitVec_eq_of_parseFirstByte_eq_done {b : UInt8} (h : parseFirstByte b = .done) :
+    b.toBitVec = 0#1 ++ b.toBitVec.setWidth 7 := by
+  exact helper₂ 7 b.toBitVec (parseFirstByte_eq_done_iff_toBitVec.1 h)
+
+/-! ### Size two -/
+
+theorem parseFirstByte_eq_oneMore_iff_toBitVec : parseFirstByte b = .oneMore ↔ b.toBitVec.extractLsb' 5 3 = 0b110#3 := by
+  simp only [parseFirstByte_eq_oneMore_iff, ← UInt8.toBitVec_inj, UInt8.toBitVec_and,
+    UInt8.toBitVec_ofNat]
+  exact helper 5 b.toBitVec 0b110#3
+
+theorem toBitVec_eq_of_parseFirstByte_eq_oneMore {b : UInt8} (h : parseFirstByte b = .oneMore) :
+    b.toBitVec = 0b110#3 ++ b.toBitVec.setWidth 5 := by
+  exact helper₂ 5 b.toBitVec (parseFirstByte_eq_oneMore_iff_toBitVec.1 h)
+
+/-! ### Size three -/
+
+theorem parseFirstByte_eq_twoMore_iff_toBitVec : parseFirstByte b = .twoMore ↔ b.toBitVec.extractLsb' 4 4 = 0b1110#4 := by
+  simp only [parseFirstByte_eq_twoMore_iff, ← UInt8.toBitVec_inj, UInt8.toBitVec_and,
+    UInt8.toBitVec_ofNat]
+  exact helper 4 b.toBitVec 0b1110#4
+
+theorem toBitVec_eq_of_parseFirstByte_eq_twoMore {b : UInt8} (h : parseFirstByte b = .twoMore) :
+    b.toBitVec = 0b1110#4 ++ b.toBitVec.setWidth 4 := by
+  exact helper₂ 4 b.toBitVec (parseFirstByte_eq_twoMore_iff_toBitVec.1 h)
+
+/-! ### Size four -/
+
+theorem parseFirstByte_eq_threeMore_iff_toBitVec : parseFirstByte b = .threeMore ↔ b.toBitVec.extractLsb' 3 5 = 0b11110#5 := by
+  simp only [parseFirstByte_eq_threeMore_iff, ← UInt8.toBitVec_inj, UInt8.toBitVec_and,
+    UInt8.toBitVec_ofNat]
+  exact helper 3 b.toBitVec 0b11110#5
+
+theorem toBitVec_eq_of_parseFirstByte_eq_threeMore {b : UInt8} (h : parseFirstByte b = .threeMore) :
+    b.toBitVec = 0b11110#5 ++ b.toBitVec.setWidth 3 := by
+  exact helper₂ 3 b.toBitVec (parseFirstByte_eq_threeMore_iff_toBitVec.1 h)
+
+/-! # `isInvalidContinuationByte` definiton & API -/
 
 @[inline]
 def isInvalidContinuationByte (b : UInt8) : Bool :=
@@ -100,223 +276,861 @@ theorem isInvalidContinutationByte_eq_false_iff {b : UInt8} :
     isInvalidContinuationByte b = false ↔ b &&& 0xc0 = 0x80 := by
   simp [isInvalidContinuationByte]
 
--- @[inline]
--- def parseLaterByte (b : UInt8) : LaterByte :=
---   if b &&& 0xc0 == 0x80 then
---     .valid (b &&& 0x3f) (UInt8.and_lt_add_one (by decide))
---   else .invalid
+theorem isInvalidContinuationByte_eq_false_iff_toBitVec {b : UInt8} :
+    isInvalidContinuationByte b = false ↔ b.toBitVec.extractLsb' 6 2 = 0b10#2 := by
+  simp only [isInvalidContinuationByte, bne_eq_false_iff_eq, ← UInt8.toBitVec_inj,
+    UInt8.toBitVec_and, UInt8.toBitVec_ofNat]
+  exact helper 6 b.toBitVec 0b10#2
 
--- theorem parseLaterByte_eq_valid (b : UInt8) (hb : b &&& 0xc0 = 0x80) :
---     parseLaterByte b = .valid (b &&& 0x3f) (UInt8.and_lt_add_one (by decide)) := by
---   grind [parseLaterByte]
+theorem toBitVec_eq_of_isInvalidContinuationByte_eq_false {b : UInt8} (hb : isInvalidContinuationByte b = false) :
+    b.toBitVec = 0b10#2 ++ b.toBitVec.setWidth 6 := by
+  exact helper₂ 6 b.toBitVec (isInvalidContinuationByte_eq_false_iff_toBitVec.1 hb)
+
+/-! # `Char.utf8Size` -/
+
+theorem Char.utf8Size_eq_one_iff {c : Char} : c.utf8Size = 1 ↔ c.val ≤ 127 := by
+  grind [utf8Size]
+
+theorem Char.utf8Size_eq_two_iff {c : Char} : c.utf8Size = 2 ↔ 128 ≤ c.val ∧ c.val ≤ 0x7ff := by
+  grind [utf8Size]
+
+theorem Char.utf8Size_eq_three_iff {c : Char} : c.utf8Size = 3 ↔ 0x7ff < c.val ∧ c.val ≤ 0xffff := by
+  grind [utf8Size]
+
+theorem Char.utf8Size_eq_four_iff {c : Char} : c.utf8Size = 4 ↔ 0xffff < c.val := by
+  grind [utf8Size]
+
+/-! # `utf8EncodeChar` -/
+
+/-! ## `utf8EncodeChar` low-level API -/
+
+theorem String.utf8EncodeChar_eq_singleton {c : Char} (h : c.utf8Size = 1) :
+    String.utf8EncodeChar c = [c.val.toUInt8] := by
+  grind [utf8EncodeChar, length_utf8EncodeChar]
+
+theorem String.utf8EncodeChar_eq_cons_cons {c : Char} (h : c.utf8Size = 2) :
+    String.utf8EncodeChar c = [(c.val >>>  6).toUInt8 &&& 0x1f ||| 0xc0, c.val.toUInt8 &&& 0x3f ||| 0x80] := by
+  grind [utf8EncodeChar, length_utf8EncodeChar]
+
+theorem String.utf8EncodeChar_eq_cons_cons_cons {c : Char} (h : c.utf8Size = 3) :
+    String.utf8EncodeChar c =
+    [(c.val >>> 12).toUInt8 &&& 0x0f ||| 0xe0,
+     (c.val >>>  6).toUInt8 &&& 0x3f ||| 0x80,
+              c.val.toUInt8 &&& 0x3f ||| 0x80] := by
+  grind [utf8EncodeChar, length_utf8EncodeChar]
+
+theorem String.utf8EncodeChar_eq_cons_cons_cons_cons {c : Char} (hc : c.utf8Size = 4) :
+    String.utf8EncodeChar c =
+    [(c.val >>> 18).toUInt8 &&& 0x07 ||| 0xf0,
+     (c.val >>> 12).toUInt8 &&& 0x3f ||| 0x80,
+     (c.val >>>  6).toUInt8 &&& 0x3f ||| 0x80,
+              c.val.toUInt8 &&& 0x3f ||| 0x80] := by
+  grind [utf8EncodeChar, length_utf8EncodeChar]
+
+/-! ## `utf8EncodeChar` BitVec API -/
+
+theorem helper₄ (s : Nat) (c : BitVec w₀) (v : BitVec w') (w : Nat) :
+    (c >>> s).setWidth (w' + w) &&& (BitVec.allOnes w).setWidth (w' + w) ||| v ++ 0#w = v ++ c.extractLsb' s w := by
+  rw [BitVec.and_setWidth_allOnes, BitVec.or_append, BitVec.zero_or, BitVec.or_zero,
+    BitVec.setWidth_shiftRight, BitVec.setWidth_extractLsb'_of_le (by simp)]
+
+/-! ### Size one -/
+
+-- TODO: possibly it makes sense to factor out this proof
+theorem String.toBitVec_getElem_utf8EncodeChar_zero_of_utf8Size_eq_one {c : Char} (h : c.utf8Size = 1) :
+    ((String.utf8EncodeChar c)[0]'(by simp [h])).toBitVec = 0#1 ++ c.val.toBitVec.extractLsb' 0 7 := by
+  have h₀ : c.val.toNat < 128 := by
+    suffices c.val.toNat ≤ 127 by omega
+    simpa [Char.utf8Size_eq_one_iff, UInt32.le_iff_toNat_le] using h
+  have h₁ : c.val.toNat < 256 := by omega
+  rw [← BitVec.toNat_inj, BitVec.toNat_append]
+  simp [utf8EncodeChar_eq_singleton h, Nat.mod_eq_of_lt h₀, Nat.mod_eq_of_lt h₁]
+
+theorem parseFirstByte_utf8EncodeChar_eq_done {c : Char} (hc : c.utf8Size = 1) :
+    parseFirstByte ((String.utf8EncodeChar c)[0]'(by simp [Char.utf8Size_pos])) = .done := by
+  rw [parseFirstByte_eq_done_iff_toBitVec, String.toBitVec_getElem_utf8EncodeChar_zero_of_utf8Size_eq_one hc,
+    BitVec.extractLsb'_append_eq_left]
+
+/-! ### Size two -/
+
+theorem String.toBitVec_getElem_utf8EncodeChar_zero_of_utf8Size_eq_two {c : Char} (h : c.utf8Size = 2) :
+    ((String.utf8EncodeChar c)[0]'(by simp [h])).toBitVec = 0b110#3 ++ c.val.toBitVec.extractLsb' 6 5 := by
+  simpa [String.utf8EncodeChar_eq_cons_cons h] using helper₄ 6 c.val.toBitVec 6#3 5
+
+theorem String.toBitVec_getElem_utf8EncodeChar_one_of_utf8Size_eq_two {c : Char} (h : c.utf8Size = 2) :
+    ((String.utf8EncodeChar c)[1]'(by simp [h])).toBitVec = 0b10#2 ++ c.val.toBitVec.extractLsb' 0 6 := by
+  simpa [String.utf8EncodeChar_eq_cons_cons h] using helper₄ 0 c.val.toBitVec 2#2 6
+
+theorem parseFirstByte_utf8EncodeChar_eq_oneMore {c : Char} (hc : c.utf8Size = 2) :
+    parseFirstByte ((String.utf8EncodeChar c)[0]'(by simp [Char.utf8Size_pos])) = .oneMore := by
+  rw [parseFirstByte_eq_oneMore_iff_toBitVec, String.toBitVec_getElem_utf8EncodeChar_zero_of_utf8Size_eq_two hc,
+    BitVec.extractLsb'_append_eq_left]
+
+theorem isInvalidContinuationByte_getElem_utf8EncodeChar_one_of_utf8Size_eq_two {c : Char} (hc : c.utf8Size = 2) :
+    isInvalidContinuationByte ((String.utf8EncodeChar c)[1]'(by simp [String.length_utf8EncodeChar, hc])) = false := by
+  rw [isInvalidContinuationByte_eq_false_iff_toBitVec, String.toBitVec_getElem_utf8EncodeChar_one_of_utf8Size_eq_two hc,
+    BitVec.extractLsb'_append_eq_left]
+
+/-! ### Size three -/
+
+theorem String.toBitVec_getElem_utf8EncodeChar_zero_of_utf8Size_eq_three {c : Char} (h : c.utf8Size = 3) :
+    ((String.utf8EncodeChar c)[0]'(by simp [h])).toBitVec = 0b1110#4 ++ c.val.toBitVec.extractLsb' 12 4 := by
+  simpa [String.utf8EncodeChar_eq_cons_cons_cons h] using helper₄ 12 c.val.toBitVec 0b1110#4 4
+
+theorem String.toBitVec_getElem_utf8EncodeChar_one_of_utf8Size_eq_three {c : Char} (h : c.utf8Size = 3) :
+    ((String.utf8EncodeChar c)[1]'(by simp [h])).toBitVec = 0b10#2 ++ c.val.toBitVec.extractLsb' 6 6 := by
+  simpa [String.utf8EncodeChar_eq_cons_cons_cons h] using helper₄ 6 c.val.toBitVec 0b10#2 6
+
+theorem String.toBitVec_getElem_utf8EncodeChar_two_of_utf8Size_eq_three {c : Char} (h : c.utf8Size = 3) :
+    ((String.utf8EncodeChar c)[2]'(by simp [h])).toBitVec = 0b10#2 ++ c.val.toBitVec.extractLsb' 0 6 := by
+  simpa [String.utf8EncodeChar_eq_cons_cons_cons h] using helper₄ 0 c.val.toBitVec 0b10#2 6
+
+theorem parseFirstByte_utf8EncodeChar_eq_twoMore {c : Char} (hc : c.utf8Size = 3) :
+    parseFirstByte ((String.utf8EncodeChar c)[0]'(by simp [Char.utf8Size_pos])) = .twoMore := by
+  rw [parseFirstByte_eq_twoMore_iff_toBitVec, String.toBitVec_getElem_utf8EncodeChar_zero_of_utf8Size_eq_three hc,
+    BitVec.extractLsb'_append_eq_left]
+
+theorem isInvalidContinuationByte_getElem_utf8EncodeChar_one_of_utf8Size_eq_three {c : Char} (hc : c.utf8Size = 3) :
+    isInvalidContinuationByte ((String.utf8EncodeChar c)[1]'(by simp [String.length_utf8EncodeChar, hc])) = false := by
+  rw [isInvalidContinuationByte_eq_false_iff_toBitVec, String.toBitVec_getElem_utf8EncodeChar_one_of_utf8Size_eq_three hc,
+    BitVec.extractLsb'_append_eq_left]
+
+theorem isInvalidContinuationByte_getElem_utf8EncodeChar_two_of_utf8Size_eq_three {c : Char} (hc : c.utf8Size = 3) :
+    isInvalidContinuationByte ((String.utf8EncodeChar c)[2]'(by simp [String.length_utf8EncodeChar, hc])) = false := by
+  rw [isInvalidContinuationByte_eq_false_iff_toBitVec, String.toBitVec_getElem_utf8EncodeChar_two_of_utf8Size_eq_three hc,
+    BitVec.extractLsb'_append_eq_left]
+
+/-! ### Size four -/
+
+theorem String.toBitVec_getElem_utf8EncodeChar_zero_of_utf8Size_eq_four {c : Char} (h : c.utf8Size = 4) :
+    ((String.utf8EncodeChar c)[0]'(by simp [h])).toBitVec = 0b11110#5 ++ c.val.toBitVec.extractLsb' 18 3 := by
+  simpa [String.utf8EncodeChar_eq_cons_cons_cons_cons h] using helper₄ 18 c.val.toBitVec 0b11110#5 3
+
+theorem String.toBitVec_getElem_utf8EncodeChar_one_of_utf8Size_eq_four {c : Char} (h : c.utf8Size = 4) :
+    ((String.utf8EncodeChar c)[1]'(by simp [h])).toBitVec = 0b10#2 ++ c.val.toBitVec.extractLsb' 12 6 := by
+  simpa [String.utf8EncodeChar_eq_cons_cons_cons_cons h] using helper₄ 12 c.val.toBitVec 0b10#2 6
+
+theorem String.toBitVec_getElem_utf8EncodeChar_two_of_utf8Size_eq_four {c : Char} (h : c.utf8Size = 4) :
+    ((String.utf8EncodeChar c)[2]'(by simp [h])).toBitVec = 0b10#2 ++ c.val.toBitVec.extractLsb' 6 6 := by
+  simpa [String.utf8EncodeChar_eq_cons_cons_cons_cons h] using helper₄ 6 c.val.toBitVec 0b10#2 6
+
+theorem String.toBitVec_getElem_utf8EncodeChar_three_of_utf8Size_eq_four {c : Char} (h : c.utf8Size = 4) :
+    ((String.utf8EncodeChar c)[3]'(by simp [h])).toBitVec = 0b10#2 ++ c.val.toBitVec.extractLsb' 0 6 := by
+  simpa [String.utf8EncodeChar_eq_cons_cons_cons_cons h] using helper₄ 0 c.val.toBitVec 0b10#2 6
+
+theorem parseFirstByte_utf8EncodeChar_eq_threeMore {c : Char} (hc : c.utf8Size = 4) :
+    parseFirstByte ((String.utf8EncodeChar c)[0]'(by simp [Char.utf8Size_pos])) = .threeMore := by
+  rw [parseFirstByte_eq_threeMore_iff_toBitVec, String.toBitVec_getElem_utf8EncodeChar_zero_of_utf8Size_eq_four hc,
+    BitVec.extractLsb'_append_eq_left]
+
+theorem isInvalidContinuationByte_getElem_utf8EncodeChar_one_of_utf8Size_eq_four {c : Char} (hc : c.utf8Size = 4) :
+    isInvalidContinuationByte ((String.utf8EncodeChar c)[1]'(by simp [String.length_utf8EncodeChar, hc])) = false := by
+  rw [isInvalidContinuationByte_eq_false_iff_toBitVec, String.toBitVec_getElem_utf8EncodeChar_one_of_utf8Size_eq_four hc,
+    BitVec.extractLsb'_append_eq_left]
+
+theorem isInvalidContinuationByte_getElem_utf8EncodeChar_two_of_utf8Size_eq_four {c : Char} (hc : c.utf8Size = 4) :
+    isInvalidContinuationByte ((String.utf8EncodeChar c)[2]'(by simp [String.length_utf8EncodeChar, hc])) = false := by
+  rw [isInvalidContinuationByte_eq_false_iff_toBitVec, String.toBitVec_getElem_utf8EncodeChar_two_of_utf8Size_eq_four hc,
+    BitVec.extractLsb'_append_eq_left]
+
+theorem isInvalidContinuationByte_getElem_utf8EncodeChar_three_of_utf8Size_eq_four {c : Char} (hc : c.utf8Size = 4) :
+    isInvalidContinuationByte ((String.utf8EncodeChar c)[3]'(by simp [String.length_utf8EncodeChar, hc])) = false := by
+  rw [isInvalidContinuationByte_eq_false_iff_toBitVec, String.toBitVec_getElem_utf8EncodeChar_three_of_utf8Size_eq_four hc,
+    BitVec.extractLsb'_append_eq_left]
+
+/-! # `assemble₁` -/
+
+theorem helper₅ {w : UInt8} (h : parseFirstByte w = .done) : w < 128 := by
+  simp only [UInt8.lt_iff_toBitVec_lt, UInt8.toBitVec_ofNat]
+  rw [toBitVec_eq_of_parseFirstByte_eq_done h]
+  simp only [Nat.reduceAdd, BitVec.lt_def, BitVec.toNat_ofNat, Nat.reducePow, Nat.reduceMod]
+  rw [BitVec.toNat_append]
+  simpa using Nat.mod_lt _ (by decide)
 
 @[inline]
-def utf8DecodeChar? (bytes : ByteArray) (i : Nat) : Option Char :=
-  if h₀ : i < bytes.size then
-    match h : parseFirstByte bytes[i] with
-    | .invalid => none -- invalid first byte
-    | .done => some ⟨bytes[i].toUInt32, ?done⟩
-    | .oneMore =>
-      let b₀ : UInt8 := bytes[i] &&& 0x1f
-      if h₁ : i +  1 < bytes.size then
-        if isInvalidContinuationByte bytes[i + 1] then
-          none
-        else
-          let b₁ := bytes[i + 1] &&& 0x3f
-          let r := (b₀.toUInt32 <<< 6) ||| b₁.toUInt32
-          if r < 0x80 then
-            none -- overlong encoding
-          else
-            some ⟨r, ?onemore⟩
-      else none
-    | .twoMore =>
-      let b₀ : UInt8 := bytes[i] &&& 0x0f
-      if h₁ : i + 2 < bytes.size then
-        if isInvalidContinuationByte bytes[i + 1] || isInvalidContinuationByte bytes[i + 2] then
-          none
-        else
-          let b₁ := bytes[i + 1] &&& 0x3f
-          let b₂ := bytes[i + 2] &&& 0x3f
-          let r := (b₀.toUInt32 <<< 12) ||| (b₁.toUInt32 <<< 6) ||| b₂.toUInt32
-          if r < 0x800 then
-            none -- overlong encoding
-          else if hr : 0xd800 ≤ r ∧ r ≤ 0xdfff then
-            none -- surrogate code point
-          else
-            some ⟨r, ?twomore⟩
-      else none
-    | .threeMore =>
-      let b₀ : UInt8 := bytes[i] &&& 0x07
-      if h₁ : i + 3 < bytes.size then
-        if isInvalidContinuationByte bytes[i + 1] || isInvalidContinuationByte bytes[i + 2] || isInvalidContinuationByte bytes[i + 3] then
-          none
-        else
-          let b₁ := bytes[i + 1] &&& 0x3f
-          let b₂ := bytes[i + 2] &&& 0x3f
-          let b₃ := bytes[i + 3] &&& 0x3f
-          let r := (b₀.toUInt32 <<< 18) ||| (b₁.toUInt32 <<< 12) ||| (b₂.toUInt32 <<< 6) ||| b₃.toUInt32
-          if h₁ : r < 0x10000 then
-            none -- overlong encoding
-          else if h₂ : 0x10ffff < r then
-            none -- out-of-range code point
-          else
-            some ⟨r, ?threemore⟩
-      else none
-  else none
+def assemble₁ (w : UInt8) (h : parseFirstByte w = .done) : Option Char :=
+  some ⟨w.toUInt32, ?done⟩
 where finally
-  case done => grind [parseFirstByte, UInt8.lt_iff_toNat_lt, UInt8.toNat_toUInt32]
+  case done =>
+    have : w < 0x80 := helper₅ h
+    refine Or.inl ?_
+    simp only [UInt8.lt_iff_toNat_lt, UInt8.reduceToNat] at this
+    simp only [UInt8.toNat_toUInt32]
+    omega
+
+theorem toBitVec_val_assemble₁ {w : UInt8} {h} {c : Char} : assemble₁ w h = some c → c.val.toBitVec = w.toBitVec.setWidth 32 := by
+  simp only [assemble₁, Option.some.injEq]
+  rintro rfl
+  rfl
+
+theorem val_assemble₁_le {w : UInt8} {h} {c : Char} (h' : assemble₁ w h = some c) : c.val ≤ 127 := by
+  have := toBitVec_val_assemble₁ h'
+  have hx := helper₅ h
+  simp only [UInt8.lt_iff_toNat_lt, UInt8.reduceToNat] at hx
+  rw [UInt32.le_iff_toBitVec_le, this, BitVec.le_def]
+  simp only [BitVec.toNat_setWidth, UInt8.toNat_toBitVec, Nat.reducePow, UInt8.toNat_mod_uInt32Size,
+    UInt32.toBitVec_ofNat, BitVec.toNat_ofNat, Nat.reduceMod]
+  omega
+
+theorem utf8Size_assemble₁ {w : UInt8} {c : Char} {h} (h : assemble₁ w h = some c) : c.utf8Size = 1 :=
+  Char.utf8Size_eq_one_iff.2 (val_assemble₁_le h)
+
+theorem assemble₁_eq_some_iff_utf8EncodeChar_eq {w : UInt8} {c : Char} :
+    (∃ h : parseFirstByte w = .done, assemble₁ w h = some c) ↔ String.utf8EncodeChar c = [w] := by
+  refine ⟨fun ⟨h₁, h₂⟩ => ?_, ?_⟩
+  · have hc := utf8Size_assemble₁ h₂
+    simp only [String.utf8EncodeChar_eq_singleton hc, List.cons.injEq, and_true]
+    simp only [assemble₁, Option.some.injEq] at h₂
+    simpa using congrArg (·.val.toUInt8) h₂ |>.symm
+  · intro h
+    have h₀ : (String.utf8EncodeChar c).length = 1 := congrArg List.length h
+    have hc : c.utf8Size = 1 := String.length_utf8EncodeChar _ ▸ h₀
+    obtain ⟨rfl⟩ : w = (String.utf8EncodeChar c)[0] := by simp [h]
+    refine ⟨parseFirstByte_utf8EncodeChar_eq_done hc, ?_⟩
+    have : c.val.toNat < 256 := by
+      simp only [Char.utf8Size_eq_one_iff, UInt32.le_iff_toNat_le, UInt32.reduceToNat] at hc
+      omega
+    simpa [String.utf8EncodeChar_eq_singleton hc, assemble₁, Char.ext_iff, ← UInt32.toNat_inj]
+
+/-! # `assemble₂` -/
+
+@[inline]
+def assemble₂Unchecked (w x : UInt8) : UInt32 :=
+  let b₀ : UInt8 := w &&& 0x1f
+  let b₁ := x &&& 0x3f
+  (b₀.toUInt32 <<< 6) ||| b₁.toUInt32
+
+@[inline]
+def assemble₂ (w x : UInt8) : Option Char :=
+  if isInvalidContinuationByte x then
+    none
+  else
+    let r := assemble₂Unchecked w x
+    if r < 0x80 then
+      none -- overlong encodinlg
+    else
+      some ⟨r, ?onemore⟩
+where finally
   case onemore =>
+    let b₀ : UInt8 := w &&& 0x1f
+    let b₁ := x &&& 0x3f
+    have hr : r = (b₀.toUInt32 <<< 6) ||| b₁.toUInt32 := rfl
     have hb₀ : b₀ < 0x20 := UInt8.and_lt_add_one (by decide)
     have hb₁ : b₁ < 0x40 := UInt8.and_lt_add_one (by decide)
     refine Or.inl ?_
-    subst r
     simp only [UInt8.lt_iff_toNat_lt, UInt8.reduceToNat] at hb₀ hb₁
-    simp only [UInt32.toNat_or, UInt32.toNat_shiftLeft, UInt8.toNat_toUInt32, UInt32.reduceToNat,
+    simp only [hr, UInt32.toNat_or, UInt32.toNat_shiftLeft, UInt8.toNat_toUInt32, UInt32.reduceToNat,
       Nat.reduceMod, Nat.reducePow]
     rw [Nat.shiftLeft_eq, Nat.mod_eq_of_lt (by omega), Nat.mul_comm, ← Nat.two_pow_add_eq_or_of_lt hb₁]
     omega
+
+theorem helper₃ {x : UInt8} (n : Nat) (hn : n < 8) :
+    (x &&& UInt8.ofNat (2 ^ n - 1)).toUInt32.toBitVec = (x.toBitVec.setWidth n).setWidth 32 := by
+  apply BitVec.eq_of_toNat_eq
+  simp only [UInt8.toUInt32_and, UInt32.toBitVec_and, UInt8.toBitVec_toUInt32, BitVec.toNat_and,
+    BitVec.toNat_setWidth, UInt8.toNat_toBitVec, Nat.reducePow, UInt8.toNat_mod_uInt32Size,
+    UInt8.toNat_ofNat']
+  have : 2 ^ n < 2 ^ 8 := Nat.pow_lt_pow_right (by decide) hn
+  rw [Nat.mod_mod_of_dvd' (by decide), Nat.mod_eq_of_lt (by omega), Nat.mod_mod_of_dvd']
+  · exact Nat.and_two_pow_sub_one_eq_mod _ _
+  · exact Nat.pow_dvd_pow (n := 32) 2 (by omega)
+
+theorem toBitVec_assemble₂Unchecked {w x : UInt8} : (assemble₂Unchecked w x).toBitVec = (w.toBitVec.setWidth 5 ++ x.toBitVec.setWidth 6).setWidth 32 := by
+  have hw : (w &&& 31).toUInt32.toBitVec = (w.toBitVec.setWidth 5).setWidth 32 := helper₃ 5 (by decide)
+  have hx : (x &&& 63).toUInt32.toBitVec = (x.toBitVec.setWidth 6).setWidth 32 := helper₃ 6 (by decide)
+  rw [assemble₂Unchecked, UInt32.toBitVec_or, UInt32.toBitVec_shiftLeft, hw, hx]
+  simpa using BitVec.setWidth_append_eq_shiftLeft_setWidth_or.symm
+
+theorem toBitVec_val_assemble₂ {w x : UInt8} (c : Char) : assemble₂ w x = some c → c.val.toBitVec = (w.toBitVec.setWidth 5 ++ x.toBitVec.setWidth 6).setWidth 32 := by
+  fun_cases assemble₂ with
+  | case1 => simp
+  | case2 => simp
+  | case3 hx r hr =>
+    simp only [Option.some.injEq, Nat.reduceAdd]
+    rintro rfl
+    subst r
+    simp [toBitVec_assemble₂Unchecked]
+
+theorem le_val_assemble₂ {w x : UInt8} {c : Char} : assemble₂ w x = some c → 128 ≤ c.val := by
+  rcases c with ⟨v, hv⟩
+  fun_cases assemble₂ with
+  | case1 => simp
+  | case2 => simp
+  | case3 hx r hr =>
+    simp only [Option.some.injEq, Char.mk.injEq]
+    rintro rfl
+    exact UInt32.not_lt.1 hr
+
+theorem val_assemble₂_le {w x : UInt8} {c : Char} (h : assemble₂ w x = some c) : c.val ≤ 2047 := by
+  rw [UInt32.le_iff_toBitVec_le, toBitVec_val_assemble₂ _ h, BitVec.le_def, BitVec.toNat_setWidth_of_le (by simp)]
+  exact Nat.le_of_lt_succ (BitVec.toNat_lt_twoPow_of_le (Nat.le_refl _))
+
+theorem utf8Size_assemble₂ {w x : UInt8} {c : Char} (h : assemble₂ w x = some c) : c.utf8Size = 2 :=
+  Char.utf8Size_eq_two_iff.2 ⟨le_val_assemble₂ h, val_assemble₂_le h⟩
+
+theorem helper₆ {c : Char} {o : Option Char} {b : BitVec 32} (hc : c.val.toBitVec = b) (h' : ∀ d, o = some d → d.val.toBitVec = b)
+    (hi : o.isSome) : o = some c := by
+  obtain rfl : c = o.get hi := by
+    refine Char.ext (UInt32.eq_of_toBitVec_eq ?_)
+    rw [hc, h' (o.get hi) (by simp)]
+  simp
+
+theorem assemble₂_eq_some_of_toBitVec {w x : UInt8} (hx : isInvalidContinuationByte x = false) {c : Char} (hc₀ : 128 ≤ c.val)
+    (hc : c.val.toBitVec = (w.toBitVec.setWidth 5 ++ x.toBitVec.setWidth 6).setWidth 32) : assemble₂ w x = some c := by
+  apply helper₆ hc toBitVec_val_assemble₂
+  fun_cases assemble₂ with
+  | case1 => simp_all
+  | case2 hx r hr =>
+    suffices 128 ≤ r.toNat ∧ r.toNat < 128 by omega
+    simp_all [← toBitVec_assemble₂Unchecked, r, UInt32.le_iff_toBitVec_le, UInt32.lt_iff_toBitVec_lt, BitVec.le_def, BitVec.lt_def]
+  | case3 hx r hr => simp
+
+theorem isInvalidContinuationByte_eq_false_of_assemble₂_eq_some {w x : UInt8} {c : Char} : assemble₂ w x = some c → isInvalidContinuationByte x = false := by
+  grind [assemble₂]
+
+theorem assemble₂_eq_some_iff_utf8EncodeChar_eq {x y : UInt8} {c : Char} :
+    parseFirstByte x = .oneMore ∧ assemble₂ x y = some c ↔ String.utf8EncodeChar c = [x, y] := by
+  refine ⟨fun ⟨h₁, h₂⟩ => ?_, ?_⟩
+  · have hc := utf8Size_assemble₂ h₂
+    rw [(String.utf8EncodeChar c).eq_getElem_of_length_eq_two (by simp [hc])]
+    simp only [List.cons.injEq, and_true, UInt8.eq_iff_toBitVec_eq]
+    refine ⟨?_, ?_⟩
+    · rw [String.toBitVec_getElem_utf8EncodeChar_zero_of_utf8Size_eq_two hc,
+        toBitVec_val_assemble₂ _ h₂, BitVec.extractLsb'_setWidth_of_le (by decide),
+        BitVec.extractLsb'_append_eq_left]
+      conv => rhs; rw [toBitVec_eq_of_parseFirstByte_eq_oneMore h₁]
+    · rw [String.toBitVec_getElem_utf8EncodeChar_one_of_utf8Size_eq_two hc,
+        toBitVec_val_assemble₂ _ h₂]
+      rw [BitVec.extractLsb'_setWidth_of_le (by decide)]
+      conv => rhs; rw [toBitVec_eq_of_isInvalidContinuationByte_eq_false (isInvalidContinuationByte_eq_false_of_assemble₂_eq_some h₂)]
+      rw [BitVec.extractLsb'_append_eq_right]
+  · intro h
+    have hc : c.utf8Size = 2 := String.length_utf8EncodeChar _ ▸ congrArg List.length h
+    have h₀ : (String.utf8EncodeChar c).length = 2 := congrArg List.length h
+    obtain ⟨rfl, rfl⟩ : x = (String.utf8EncodeChar c)[0] ∧ y = (String.utf8EncodeChar c)[1] := by simp [h]
+    refine ⟨parseFirstByte_utf8EncodeChar_eq_oneMore hc, ?_⟩
+    apply assemble₂_eq_some_of_toBitVec
+    · apply isInvalidContinuationByte_getElem_utf8EncodeChar_one_of_utf8Size_eq_two hc
+    · rw [Char.utf8Size_eq_two_iff] at hc
+      exact hc.1
+    · rw [String.toBitVec_getElem_utf8EncodeChar_zero_of_utf8Size_eq_two hc,
+        String.toBitVec_getElem_utf8EncodeChar_one_of_utf8Size_eq_two hc,
+        BitVec.setWidth_append_eq_right, BitVec.setWidth_append_eq_right,
+        extractLsb'_append_extractLsb'_eq_extractLsb'_better (by simp),
+        ← BitVec.setWidth_eq_extractLsb' (by simp),
+        BitVec.setWidth_setWidth_eq_self]
+      simpa [BitVec.lt_def, UInt32.le_iff_toNat_le] using Nat.lt_succ_iff.2 (Char.utf8Size_eq_two_iff.1 hc).2
+
+/-! # `assemble₃` -/
+
+@[inline]
+def assemble₃Unchecked (w x y : UInt8) : UInt32 :=
+  let b₀ : UInt8 := w &&& 0x0f
+  let b₁ := x &&& 0x3f
+  let b₂ := y &&& 0x3f
+  (b₀.toUInt32 <<< 12) ||| (b₁.toUInt32 <<< 6) ||| b₂.toUInt32
+
+@[inline]
+def assemble₃ (w x y : UInt8) : Option Char :=
+  if isInvalidContinuationByte x || isInvalidContinuationByte y then
+    none
+  else
+    let r := assemble₃Unchecked w x y
+    if r < 0x800 then
+      none -- overlong encoding
+    else if hr : 0xd800 ≤ r ∧ r ≤ 0xdfff then
+      none -- surrogate code point
+    else
+      some ⟨r, ?twomore⟩
+where finally
   case twomore =>
+    let b₀ : UInt8 := w &&& 0x0f
+    let b₁ := x &&& 0x3f
+    let b₂ := y &&& 0x3f
     have hb₀ : b₀ < 0x10 := UInt8.and_lt_add_one (by decide)
     have hb₁ : b₁ < 0x40 := UInt8.and_lt_add_one (by decide)
     have hb₂ : b₂ < 0x40 := UInt8.and_lt_add_one (by decide)
+    have hr' : r = (b₀.toUInt32 <<< 12) ||| (b₁.toUInt32 <<< 6) ||| b₂.toUInt32 := rfl
     simp only [UInt8.lt_iff_toNat_lt, UInt8.reduceToNat] at hb₀ hb₁ hb₂
     simp only [Decidable.not_and_iff_not_or_not, UInt32.not_le] at hr
     rcases hr with (hr|hr)
     · exact Or.inl hr
     · refine Or.inr ⟨hr, ?_⟩
       subst r
-      simp only [UInt32.toNat_or, UInt32.toNat_shiftLeft, UInt8.toNat_toUInt32, UInt32.reduceToNat,
+      simp only [hr', UInt32.toNat_or, UInt32.toNat_shiftLeft, UInt8.toNat_toUInt32, UInt32.reduceToNat,
         Nat.reduceMod, Nat.reducePow]
       rw [Nat.shiftLeft_eq, Nat.shiftLeft_eq, Nat.mod_eq_of_lt (by omega), Nat.mod_eq_of_lt (by omega),
         Nat.mul_comm _ (2 ^ _), Nat.mul_comm _ (2 ^ _), Nat.or_assoc, ← Nat.two_pow_add_eq_or_of_lt (b := b₂.toNat) hb₂,
           ← Nat.two_pow_add_eq_or_of_lt (by omega)]
       omega
+
+theorem toBitVec_assemble₃Unchecked {w x y : UInt8} : (assemble₃Unchecked w x y).toBitVec =
+    (w.toBitVec.setWidth 4 ++ x.toBitVec.setWidth 6 ++ y.toBitVec.setWidth 6).setWidth 32 := by
+  have hw : (w &&& 15).toUInt32.toBitVec = (w.toBitVec.setWidth 4).setWidth 32 := helper₃ 4 (by decide)
+  have hx : (x &&& 63).toUInt32.toBitVec = (x.toBitVec.setWidth 6).setWidth 32 := helper₃ 6 (by decide)
+  have hy : (y &&& 63).toUInt32.toBitVec = (y.toBitVec.setWidth 6).setWidth 32 := helper₃ 6 (by decide)
+  rw [assemble₃Unchecked, UInt32.toBitVec_or, UInt32.toBitVec_or, UInt32.toBitVec_shiftLeft, UInt32.toBitVec_shiftLeft,
+    hw, hx, hy, BitVec.setWidth_append_append_eq_shiftLeft_setWidth_or]
+  simp
+
+theorem toBitVec_val_assemble₃ {w x y : UInt8} (c : Char) : assemble₃ w x y = some c →
+    c.val.toBitVec = (w.toBitVec.setWidth 4 ++ x.toBitVec.setWidth 6 ++ y.toBitVec.setWidth 6).setWidth 32 := by
+  fun_cases assemble₃ with
+  | case1 => simp
+  | case2 => simp
+  | case3 => simp
+  | case4 hx r hr =>
+    simp only [Option.some.injEq, Nat.reduceAdd]
+    rintro rfl
+    subst r
+    simp [toBitVec_assemble₃Unchecked]
+
+theorem le_val_assemble₃ {w x y : UInt8} {c : Char} : assemble₃ w x y = some c → 0x800 ≤ c.val := by
+  rcases c with ⟨v, hv⟩
+  fun_cases assemble₃ with
+  | case1 => simp
+  | case2 => simp
+  | case3 => simp
+  | case4 hx r hr =>
+    simp only [Option.some.injEq, Char.mk.injEq]
+    rintro rfl
+    exact UInt32.not_lt.1 hr
+
+theorem val_assemble₃_le {w x y : UInt8} {c : Char} (h : assemble₃ w x y = some c) : c.val ≤ 0xffff := by
+  rw [UInt32.le_iff_toBitVec_le, toBitVec_val_assemble₃ _ h, BitVec.le_def, BitVec.toNat_setWidth_of_le (by simp)]
+  exact Nat.le_of_lt_succ (BitVec.toNat_lt_twoPow_of_le (Nat.le_refl _))
+
+theorem utf8Size_assemble₃ {w x y : UInt8} {c : Char} (h : assemble₃ w x y = some c) : c.utf8Size = 3 :=
+  Char.utf8Size_eq_three_iff.2 ⟨le_val_assemble₃ h, val_assemble₃_le h⟩
+
+theorem assemble₃_eq_some_of_toBitVec {w x y : UInt8} (hx : isInvalidContinuationByte x = false)
+    (hy : isInvalidContinuationByte y = false) {c : Char} (hc₀ : 0x800 ≤ c.val)
+    (hc : c.val.toBitVec = (w.toBitVec.setWidth 4 ++ x.toBitVec.setWidth 6 ++ y.toBitVec.setWidth 6).setWidth 32) :
+    assemble₃ w x y = some c := by
+  apply helper₆ hc toBitVec_val_assemble₃
+  fun_cases assemble₃ with
+  | case1 => simp_all
+  | case2 hx r hr =>
+    suffices 0x800 ≤ (assemble₃Unchecked w x y).toNat ∧ (assemble₃Unchecked w x y).toNat < 0x800 by omega
+    simp_all [← toBitVec_assemble₃Unchecked, r, UInt32.le_iff_toBitVec_le, UInt32.lt_iff_toBitVec_lt, BitVec.le_def, BitVec.lt_def]
+  | case3 hx r hr hr' =>
+    have hcv := c.valid
+    suffices ((55296 ≤ r.toNat ∧ r.toNat ≤ 57343) ∧ (r.toNat < 55296 ∨ (57343 < r.toNat ∧ r.toNat < 1114112))) by omega
+    simp_all [UInt32.isValidChar, Nat.isValidChar, ← toBitVec_assemble₃Unchecked, r, UInt32.le_iff_toBitVec_le, UInt32.lt_iff_toBitVec_lt,
+      BitVec.le_def, BitVec.lt_def, ← BitVec.toNat_inj]
+  | case4 => simp
+
+theorem isInvalidContinuationByte_eq_false_of_assemble₃_eq_some_left {w x y : UInt8} {c : Char} : assemble₃ w x y = some c → isInvalidContinuationByte x = false := by
+  grind [assemble₃]
+
+theorem isInvalidContinuationByte_eq_false_of_assemble₃_eq_some_right {w x y : UInt8} {c : Char} : assemble₃ w x y = some c → isInvalidContinuationByte y = false := by
+  grind [assemble₃]
+
+theorem assemble₃_eq_some_iff_utf8EncodeChar_eq {w x y : UInt8} {c : Char} :
+    parseFirstByte w = .twoMore ∧ assemble₃ w x y = some c ↔ String.utf8EncodeChar c = [w, x, y] := by
+  refine ⟨fun ⟨h₁, h₂⟩ => ?_, ?_⟩
+  · have hc := utf8Size_assemble₃ h₂
+    rw [(String.utf8EncodeChar c).eq_getElem_of_length_eq_three (by simp [hc])]
+    simp only [List.cons.injEq, UInt8.eq_iff_toBitVec_eq, and_true]
+    refine ⟨?_, ?_, ?_⟩
+    · rw [String.toBitVec_getElem_utf8EncodeChar_zero_of_utf8Size_eq_three hc,
+        toBitVec_val_assemble₃ _ h₂, BitVec.extractLsb'_setWidth_of_le (by decide),
+        BitVec.append_assoc, BitVec.cast_eq, BitVec.extractLsb'_append_eq_left,
+        ← toBitVec_eq_of_parseFirstByte_eq_twoMore h₁]
+    · rw [String.toBitVec_getElem_utf8EncodeChar_one_of_utf8Size_eq_three hc,
+        toBitVec_val_assemble₃ _ h₂, BitVec.extractLsb'_setWidth_of_le (by decide),
+        BitVec.extractLsb'_append_eq_of_le (by decide), BitVec.extractLsb'_append_eq_right,
+        ← toBitVec_eq_of_isInvalidContinuationByte_eq_false (isInvalidContinuationByte_eq_false_of_assemble₃_eq_some_left h₂)]
+    · rw [String.toBitVec_getElem_utf8EncodeChar_two_of_utf8Size_eq_three hc,
+        toBitVec_val_assemble₃ _ h₂, BitVec.extractLsb'_setWidth_of_le (by decide),
+        BitVec.extractLsb'_append_eq_right,
+        ← toBitVec_eq_of_isInvalidContinuationByte_eq_false (isInvalidContinuationByte_eq_false_of_assemble₃_eq_some_right h₂)]
+  · intro h
+    have h₀ : (String.utf8EncodeChar c).length = 3 := congrArg List.length h
+    have hc : c.utf8Size = 3 := String.length_utf8EncodeChar _ ▸ h₀
+    obtain ⟨rfl, rfl, rfl⟩ : w = (String.utf8EncodeChar c)[0] ∧ x = (String.utf8EncodeChar c)[1] ∧
+      y = (String.utf8EncodeChar c)[2] := by simp [h]
+    refine ⟨parseFirstByte_utf8EncodeChar_eq_twoMore hc, ?_⟩
+    apply assemble₃_eq_some_of_toBitVec
+    · apply isInvalidContinuationByte_getElem_utf8EncodeChar_one_of_utf8Size_eq_three hc
+    · apply isInvalidContinuationByte_getElem_utf8EncodeChar_two_of_utf8Size_eq_three hc
+    · simp [Char.utf8Size_eq_three_iff, UInt32.lt_iff_toNat_lt] at hc
+      exact UInt32.le_iff_toNat_le.2 (by simp; omega)
+    · rw [String.toBitVec_getElem_utf8EncodeChar_zero_of_utf8Size_eq_three hc,
+        String.toBitVec_getElem_utf8EncodeChar_one_of_utf8Size_eq_three hc,
+        String.toBitVec_getElem_utf8EncodeChar_two_of_utf8Size_eq_three hc,
+        BitVec.setWidth_append_eq_right, BitVec.setWidth_append_eq_right, BitVec.setWidth_append_eq_right,
+        extractLsb'_append_extractLsb'_eq_extractLsb'_better (by simp),
+        extractLsb'_append_extractLsb'_eq_extractLsb'_better (by simp),
+        ← BitVec.setWidth_eq_extractLsb' (by simp), BitVec.setWidth_setWidth_eq_self]
+      simpa [BitVec.lt_def, UInt32.le_iff_toNat_le] using Nat.lt_succ_iff.2 (Char.utf8Size_eq_three_iff.1 hc).2
+
+/-! # `assemble₄` -/
+
+@[inline]
+def assemble₄Unchecked (w x y z : UInt8) : UInt32 :=
+  let b₀ : UInt8 := w &&& 0x07
+  let b₁ := x &&& 0x3f
+  let b₂ := y &&& 0x3f
+  let b₃ := z &&& 0x3f
+  (b₀.toUInt32 <<< 18) ||| (b₁.toUInt32 <<< 12) ||| (b₂.toUInt32 <<< 6) ||| b₃.toUInt32
+
+@[inline]
+def assemble₄ (w x y z : UInt8) : Option Char :=
+  if isInvalidContinuationByte x || isInvalidContinuationByte y || isInvalidContinuationByte z then
+    none
+  else
+    let r := assemble₄Unchecked w x y z
+    if h₁ : r < 0x10000 then
+      none -- overlong encoding
+    else if h₂ : 0x10ffff < r then
+      none -- out-of-range code point
+    else
+      some ⟨r, ?threemore⟩
+where finally
   case threemore =>
-    have hb₀ : b₀ < 0x08 := UInt8.and_lt_add_one (by decide)
-    have hb₁ : b₁ < 0x40 := UInt8.and_lt_add_one (by decide)
-    have hb₂ : b₂ < 0x40 := UInt8.and_lt_add_one (by decide)
-    have hb₃ : b₃ < 0x40 := UInt8.and_lt_add_one (by decide)
-    simp only [UInt8.lt_iff_toNat_lt, UInt8.reduceToNat] at hb₀ hb₁ hb₂ hb₃
     simp only [UInt32.not_lt, UInt32.le_iff_toNat_le, UInt32.reduceToNat] at h₁ h₂
     exact Or.inr ⟨by omega, by omega⟩
 
-def utf8DecodeChar (bytes : ByteArray) (i : Nat) (h : (utf8DecodeChar? bytes i).isSome) : Char :=
-  (utf8DecodeChar? bytes i).get h
+theorem toBitVec_assemble₄Unchecked {w x y z : UInt8} : (assemble₄Unchecked w x y z).toBitVec =
+    (w.toBitVec.setWidth 3 ++ x.toBitVec.setWidth 6 ++ y.toBitVec.setWidth 6 ++ z.toBitVec.setWidth 6).setWidth 32 := by
+  have hw : (w &&& 7).toUInt32.toBitVec = (w.toBitVec.setWidth 3).setWidth 32 := helper₃ 3 (by decide)
+  have hx : (x &&& 63).toUInt32.toBitVec = (x.toBitVec.setWidth 6).setWidth 32 := helper₃ 6 (by decide)
+  have hy : (y &&& 63).toUInt32.toBitVec = (y.toBitVec.setWidth 6).setWidth 32 := helper₃ 6 (by decide)
+  have hz : (z &&& 63).toUInt32.toBitVec = (z.toBitVec.setWidth 6).setWidth 32 := helper₃ 6 (by decide)
+  rw [assemble₄Unchecked, UInt32.toBitVec_or, UInt32.toBitVec_or, UInt32.toBitVec_or, UInt32.toBitVec_shiftLeft,
+    UInt32.toBitVec_shiftLeft, UInt32.toBitVec_shiftLeft, hw, hx, hy, hz, BitVec.setWidth_append_append_append_eq_shiftLeft_setWidth_or]
+  simp
+
+theorem toBitVec_val_assemble₄ {w x y z : UInt8} (c : Char) : assemble₄ w x y z = some c →
+    c.val.toBitVec = (w.toBitVec.setWidth 3 ++ x.toBitVec.setWidth 6 ++ y.toBitVec.setWidth 6 ++ z.toBitVec.setWidth 6).setWidth 32 := by
+  fun_cases assemble₄ with
+  | case1 => simp
+  | case2 => simp
+  | case3 => simp
+  | case4 hx r hr =>
+    simp only [Option.some.injEq, Nat.reduceAdd]
+    rintro rfl
+    subst r
+    simp [toBitVec_assemble₄Unchecked]
+
+theorem le_val_assemble₄ {w x y z : UInt8} {c : Char} : assemble₄ w x y z = some c → 0xffff < c.val := by
+  rcases c with ⟨v, hv⟩
+  fun_cases assemble₄ with
+  | case1 => simp
+  | case2 => simp
+  | case3 => simp
+  | case4 hx r hr =>
+    simp only [Option.some.injEq, Char.mk.injEq]
+    rintro rfl
+    have := UInt32.not_lt.1 hr
+    simp only [UInt32.le_iff_toNat_le, UInt32.reduceToNat] at this
+    simp only [UInt32.lt_iff_toNat_lt, UInt32.reduceToNat, gt_iff_lt]
+    omega
+
+theorem utf8Size_assemble₄ {w x y z : UInt8} {c : Char} (h : assemble₄ w x y z = some c) : c.utf8Size = 4 :=
+  Char.utf8Size_eq_four_iff.2 (le_val_assemble₄ h)
+
+theorem assemble₄_eq_some_of_toBitVec {w x y z : UInt8} (hx : isInvalidContinuationByte x = false)
+    (hy : isInvalidContinuationByte y = false) (hz : isInvalidContinuationByte z = false) {c : Char} (hc₀ : 0x10000 ≤ c.val)
+    (hc : c.val.toBitVec = (w.toBitVec.setWidth 3 ++ x.toBitVec.setWidth 6 ++ y.toBitVec.setWidth 6 ++ z.toBitVec.setWidth 6).setWidth 32) :
+    assemble₄ w x y z = some c := by
+  apply helper₆ hc toBitVec_val_assemble₄
+  fun_cases assemble₄ with
+  | case1 => simp_all
+  | case2 hx r hr =>
+    suffices 0x10000 ≤ (assemble₄Unchecked w x y z).toNat ∧ (assemble₄Unchecked w x y z).toNat < 0x10000 by omega
+    simp_all [← toBitVec_assemble₄Unchecked, r, UInt32.le_iff_toBitVec_le, UInt32.lt_iff_toBitVec_lt, BitVec.le_def, BitVec.lt_def]
+  | case3 hx r hr hr' =>
+    have hcv := c.valid
+    suffices (1114111 < r.toNat ∧ (r.toNat < 55296 ∨ (57343 < r.toNat ∧ r.toNat < 1114112))) by omega
+    simp_all [UInt32.isValidChar, Nat.isValidChar, ← toBitVec_assemble₄Unchecked, r, UInt32.le_iff_toBitVec_le, UInt32.lt_iff_toBitVec_lt,
+      BitVec.le_def, BitVec.lt_def, ← BitVec.toNat_inj]
+  | case4 => simp
+
+theorem isInvalidContinuationByte_eq_false_of_assemble₄_eq_some_left {w x y z : UInt8} {c : Char} : assemble₄ w x y z = some c → isInvalidContinuationByte x = false := by
+  grind [assemble₄]
+
+theorem isInvalidContinuationByte_eq_false_of_assemble₄_eq_some_middle {w x y z : UInt8} {c : Char} : assemble₄ w x y z = some c → isInvalidContinuationByte y = false := by
+  grind [assemble₄]
+
+theorem isInvalidContinuationByte_eq_false_of_assemble₄_eq_some_right {w x y z : UInt8} {c : Char} : assemble₄ w x y z = some c → isInvalidContinuationByte z = false := by
+  grind [assemble₄]
+
+theorem Char.toNat_val_le {c : Char} : c.val.toNat ≤ 0x10ffff := by
+  have := c.valid
+  simp [UInt32.isValidChar, Nat.isValidChar] at this
+  omega
+
+theorem assemble₄_eq_some_iff_utf8EncodeChar_eq {w x y z : UInt8} {c : Char} :
+    parseFirstByte w = .threeMore ∧ assemble₄ w x y z = some c ↔ String.utf8EncodeChar c = [w, x, y, z] := by
+  refine ⟨fun ⟨h₁, h₂⟩ => ?_, ?_⟩
+  · have hc := utf8Size_assemble₄ h₂
+    rw [(String.utf8EncodeChar c).eq_getElem_of_length_eq_four (by simp [hc])]
+    simp only [List.cons.injEq, UInt8.eq_iff_toBitVec_eq, and_true]
+    refine ⟨?_, ?_, ?_, ?_⟩
+    · rw [String.toBitVec_getElem_utf8EncodeChar_zero_of_utf8Size_eq_four hc,
+        toBitVec_val_assemble₄ _ h₂, BitVec.extractLsb'_setWidth_of_le (by decide),
+        BitVec.append_assoc, BitVec.cast_eq, BitVec.append_assoc, BitVec.cast_eq,
+        BitVec.extractLsb'_append_eq_left,
+        ← toBitVec_eq_of_parseFirstByte_eq_threeMore h₁]
+    · rw [String.toBitVec_getElem_utf8EncodeChar_one_of_utf8Size_eq_four hc,
+        toBitVec_val_assemble₄ _ h₂, BitVec.extractLsb'_setWidth_of_le (by decide),
+        BitVec.extractLsb'_append_eq_of_le (by decide), BitVec.extractLsb'_append_eq_of_le (by decide),
+        BitVec.extractLsb'_append_eq_right,
+        ← toBitVec_eq_of_isInvalidContinuationByte_eq_false (isInvalidContinuationByte_eq_false_of_assemble₄_eq_some_left h₂)]
+    · rw [String.toBitVec_getElem_utf8EncodeChar_two_of_utf8Size_eq_four hc,
+        toBitVec_val_assemble₄ _ h₂, BitVec.extractLsb'_setWidth_of_le (by decide),
+        BitVec.extractLsb'_append_eq_of_le (by decide), BitVec.extractLsb'_append_eq_right,
+        ← toBitVec_eq_of_isInvalidContinuationByte_eq_false (isInvalidContinuationByte_eq_false_of_assemble₄_eq_some_middle h₂)]
+    · rw [String.toBitVec_getElem_utf8EncodeChar_three_of_utf8Size_eq_four hc,
+        toBitVec_val_assemble₄ _ h₂, BitVec.extractLsb'_setWidth_of_le (by decide),
+        BitVec.extractLsb'_append_eq_right,
+        ← toBitVec_eq_of_isInvalidContinuationByte_eq_false (isInvalidContinuationByte_eq_false_of_assemble₄_eq_some_right h₂)]
+  · intro h
+    have h₀ : (String.utf8EncodeChar c).length = 4 := congrArg List.length h
+    have hc : c.utf8Size = 4 :=  String.length_utf8EncodeChar _ ▸ h₀
+    obtain ⟨rfl, rfl, rfl, rfl⟩ :
+      w = (String.utf8EncodeChar c)[0] ∧ x = (String.utf8EncodeChar c)[1] ∧ y = (String.utf8EncodeChar c)[2]
+        ∧ z = (String.utf8EncodeChar c)[3] := by simp [h]
+    refine ⟨parseFirstByte_utf8EncodeChar_eq_threeMore hc, ?_⟩
+    apply assemble₄_eq_some_of_toBitVec
+    · apply isInvalidContinuationByte_getElem_utf8EncodeChar_one_of_utf8Size_eq_four hc
+    · apply isInvalidContinuationByte_getElem_utf8EncodeChar_two_of_utf8Size_eq_four hc
+    · apply isInvalidContinuationByte_getElem_utf8EncodeChar_three_of_utf8Size_eq_four hc
+    · simp [Char.utf8Size_eq_four_iff, UInt32.lt_iff_toNat_lt] at hc
+      exact UInt32.le_iff_toNat_le.2 (by simp; omega)
+    · rw [String.toBitVec_getElem_utf8EncodeChar_zero_of_utf8Size_eq_four hc,
+        String.toBitVec_getElem_utf8EncodeChar_one_of_utf8Size_eq_four hc,
+        String.toBitVec_getElem_utf8EncodeChar_two_of_utf8Size_eq_four hc,
+        String.toBitVec_getElem_utf8EncodeChar_three_of_utf8Size_eq_four hc,
+        BitVec.setWidth_append_eq_right, BitVec.setWidth_append_eq_right, BitVec.setWidth_append_eq_right,
+        BitVec.setWidth_append_eq_right,
+        extractLsb'_append_extractLsb'_eq_extractLsb'_better (by simp),
+        extractLsb'_append_extractLsb'_eq_extractLsb'_better (by simp),
+        extractLsb'_append_extractLsb'_eq_extractLsb'_better (by simp),
+        ← BitVec.setWidth_eq_extractLsb' (by simp), BitVec.setWidth_setWidth_eq_self]
+      have := c.toNat_val_le
+      simp only [Nat.reduceAdd, BitVec.lt_def, UInt32.toNat_toBitVec, BitVec.toNat_twoPow,
+        Nat.reducePow, Nat.reduceMod, gt_iff_lt]
+      omega
+
+/- # `utf8DecodeChar?` -/
+
+@[inline]
+def utf8DecodeChar? (bytes : ByteArray) (i : Nat) : Option Char :=
+  if h₀ : i < bytes.size then
+    match h : parseFirstByte bytes[i] with
+    | .invalid => none -- invalid first byte
+    | .done => assemble₁ bytes[i] h
+    | .oneMore =>
+      if h₁ : i + 1 < bytes.size then
+        assemble₂ bytes[i] bytes[i + 1]
+      else
+        none
+    | .twoMore =>
+      if h₁ : i + 2 < bytes.size then
+        assemble₃ bytes[i] bytes[i + 1] bytes[i + 2]
+      else none
+    | .threeMore =>
+      if h₁ : i + 3 < bytes.size then
+        assemble₄ bytes[i] bytes[i + 1] bytes[i + 2] bytes[i + 3]
+      else none
+  else none
+
+/-! # `utf8DecodeChar?` low-level API -/
+
+theorem parseFirstByte_eq_done_of_utf8DecodeChar?_eq_some {b : ByteArray} {i : Nat} {c : Char}
+    (h : utf8DecodeChar? b i = some c) (hc : c.utf8Size = 1) (h') :
+    parseFirstByte (b[i]'h') = .done := by
+  revert h
+  fun_cases utf8DecodeChar? with
+  | case1 => simp
+  | case2 => simp_all
+  | case3 => exact (by omega) ∘ utf8Size_assemble₂
+  | case4 => simp
+  | case5 => exact (by omega) ∘ utf8Size_assemble₃
+  | case6 => simp
+  | case7 => exact (by omega) ∘ utf8Size_assemble₄
+  | case8 => simp
+  | case9 => simp
+
+theorem parseFirstByte_eq_oneMore_of_utf8DecodeChar?_eq_some {b : ByteArray} {i : Nat} {c : Char}
+    (h : utf8DecodeChar? b i = some c) (hc : c.utf8Size = 2) (h') :
+    parseFirstByte (b[i]'h') = .oneMore := by
+  revert h
+  fun_cases utf8DecodeChar? with
+  | case1 => simp
+  | case2 => exact (by omega) ∘ utf8Size_assemble₁
+  | case3 => simp_all
+  | case4 => simp
+  | case5 => exact (by omega) ∘ utf8Size_assemble₃
+  | case6 => simp
+  | case7 => exact (by omega) ∘ utf8Size_assemble₄
+  | case8 => simp
+  | case9 => simp
+
+theorem parseFirstByte_eq_twoMore_of_utf8DecodeChar?_eq_some {b : ByteArray} {i : Nat} {c : Char}
+    (h : utf8DecodeChar? b i = some c) (hc : c.utf8Size = 3) (h') :
+    parseFirstByte (b[i]'h') = .twoMore := by
+  revert h
+  fun_cases utf8DecodeChar? with
+  | case1 => simp
+  | case2 => exact (by omega) ∘ utf8Size_assemble₁
+  | case3 => exact (by omega) ∘ utf8Size_assemble₂
+  | case4 => simp
+  | case5 => simp_all
+  | case6 => simp
+  | case7 => exact (by omega) ∘ utf8Size_assemble₄
+  | case8 => simp
+  | case9 => simp
+
+theorem parseFirstByte_eq_threeMore_of_utf8DecodeChar?_eq_some {b : ByteArray} {i : Nat} {c : Char}
+    (h : utf8DecodeChar? b i = some c) (hc : c.utf8Size = 4) (h') :
+    parseFirstByte (b[i]'h') = .threeMore := by
+  revert h
+  fun_cases utf8DecodeChar? with
+  | case1 => simp
+  | case2 => exact (by omega) ∘ utf8Size_assemble₁
+  | case3 => exact (by omega) ∘ utf8Size_assemble₂
+  | case4 => simp
+  | case5 => exact (by omega) ∘ utf8Size_assemble₃
+  | case6 => simp
+  | case7 => simp_all
+  | case8 => simp
+  | case9 => simp
+
+theorem utf8Size_le_of_utf8DecodeChar?_eq_some {b : ByteArray} {c : Char} :
+    utf8DecodeChar? b 0 = some c → c.utf8Size ≤ b.size := by
+  fun_cases utf8DecodeChar? with
+  | case1 => simp
+  | case2 => exact (by omega) ∘ utf8Size_assemble₁
+  | case3 => exact (by omega) ∘ utf8Size_assemble₂
+  | case4 => simp
+  | case5 => exact (by omega) ∘ utf8Size_assemble₃
+  | case6 => simp
+  | case7 => exact (by omega) ∘ utf8Size_assemble₄
+  | case8 => simp
+  | case9 => simp
+
+theorem utf8DecodeChar?_eq_assemble₁ {b : ByteArray} (hb : 1 ≤ b.size) (h : parseFirstByte b[0] = .done) :
+    utf8DecodeChar? b 0 = assemble₁ b[0] h := by
+  fun_cases utf8DecodeChar?
+  all_goals try (simp_all; done)
+  all_goals omega
+
+theorem utf8DecodeChar?_eq_assemble₂ {b : ByteArray} (hb : 2 ≤ b.size) (h : parseFirstByte b[0] = .oneMore) :
+    utf8DecodeChar? b 0 = assemble₂ b[0] b[1] := by
+  fun_cases utf8DecodeChar?
+  all_goals try (simp_all; done)
+  all_goals omega
+
+theorem utf8DecodeChar?_eq_assemble₃ {b : ByteArray} (hb : 3 ≤ b.size) (h : parseFirstByte b[0] = .twoMore) :
+    utf8DecodeChar? b 0 = assemble₃ b[0] b[1] b[2] := by
+  fun_cases utf8DecodeChar?
+  all_goals try (simp_all; done)
+  all_goals omega
+
+theorem utf8DecodeChar?_eq_assemble₄ {b : ByteArray} (hb : 4 ≤ b.size) (h : parseFirstByte b[0] = .threeMore) :
+    utf8DecodeChar? b 0 = assemble₄ b[0] b[1] b[2] b[3] := by
+  fun_cases utf8DecodeChar?
+  all_goals try (simp_all; done)
+  all_goals omega
+
+theorem utf8DecodeChar?_append_eq_assemble₁ {l : List UInt8} {b : ByteArray} (hl : l.length = 1) (h : parseFirstByte l[0] = .done) :
+    utf8DecodeChar? (l.toByteArray ++ b) 0 = assemble₁ l[0] h := by
+  have : (l.toByteArray ++ b)[0]'(by simp [hl]; omega) = l[0] := by
+    rw [ByteArray.getElem_append_left (by simp [hl]), List.getElem_toByteArray]
+  rw [utf8DecodeChar?_eq_assemble₁ (by simp [hl])] <;> simp [this, h]
+
+theorem utf8DecodeChar?_append_eq_assemble₂ {l : List UInt8} {b : ByteArray} (hl : l.length = 2) (h : parseFirstByte l[0] = .oneMore) :
+    utf8DecodeChar? (l.toByteArray ++ b) 0 = assemble₂ l[0] l[1] := by
+  rw [utf8DecodeChar?_eq_assemble₂ (by simp [hl])]
+  all_goals repeat rw [ByteArray.getElem_append_left (by simp [hl])]
+  all_goals repeat rw [List.getElem_toByteArray]
+  assumption
+
+theorem utf8DecodeChar?_append_eq_assemble₃ {l : List UInt8} {b : ByteArray} (hl : l.length = 3) (h : parseFirstByte l[0] = .twoMore) :
+    utf8DecodeChar? (l.toByteArray ++ b) 0 = assemble₃ l[0] l[1] l[2] := by
+  rw [utf8DecodeChar?_eq_assemble₃ (by simp [hl])]
+  all_goals repeat rw [ByteArray.getElem_append_left (by simp [hl])]
+  all_goals repeat rw [List.getElem_toByteArray]
+  assumption
+
+theorem utf8DecodeChar?_append_eq_assemble₄ {l : List UInt8} {b : ByteArray} (hl : l.length = 4) (h : parseFirstByte l[0] = .threeMore) :
+    utf8DecodeChar? (l.toByteArray ++ b) 0 = assemble₄ l[0] l[1] l[2] l[3] := by
+  rw [utf8DecodeChar?_eq_assemble₄ (by simp [hl])]
+  all_goals repeat rw [ByteArray.getElem_append_left (by simp [hl])]
+  all_goals repeat rw [List.getElem_toByteArray]
+  assumption
+
+/-!
+# Main theorems
+
+`utf8DecodeChar?_utf8EncodeChar_append` and `toByteArray_of_utf8DecodeChar?_eq_some` are the two main results that together
+imply that UTF-8 encoding and decoding are inverse.
+-/
 
 theorem utf8DecodeChar?_utf8EncodeChar_append {b : ByteArray} {c : Char} :
     utf8DecodeChar? ((String.utf8EncodeChar c).toByteArray ++ b) 0 = some c := by
-  fun_cases String.utf8EncodeChar c with
-  | case1 v h =>
-    rw [utf8DecodeChar?, dif_pos (by simp; grind [Char.utf8Size_pos])]
-    have : parseFirstByte ([v.toUInt8].toByteArray ++ b)[0] = .done := by
-      rw [parseFirstByte_eq_done]
-      simp [UInt8.le_iff_toNat_le, UInt32.le_iff_toNat_le] at h ⊢
-      grind
-    split <;> rename_i h' <;> try (simp_all; done)
-    · simp only [Option.some.injEq]
-      ext
-      simp
-      grind
-  | case2 v h₁ h₂ =>
-    rw [utf8DecodeChar?, dif_pos (by simp; grind [Char.utf8Size_pos])]
-    sorry
-    -- rw [parseFirstByte_eq_oneMore]
-    -- · simp only
-    --   rw [dif_pos (by simp; grind)]
-    --   simp only [Nat.zero_add, List.size_toByteArray, List.length_cons, List.length_nil,
-    --     Nat.reduceAdd, Nat.lt_add_one, ByteArray.getElem_append_left, List.getElem_toByteArray,
-    --     List.getElem_cons_succ, List.getElem_cons_zero, Nat.zero_lt_succ, UInt8.toUInt32_and,
-    --     UInt8.toUInt32_or, UInt32.toUInt32_toUInt8, Nat.reduceLT, UInt8.toUInt32_ofNat]
-    --   rw [parseLaterByte_eq_valid]
-    --   · simp only [UInt8.toUInt32_and, UInt8.toUInt32_or, UInt32.toUInt32_toUInt8, Nat.reduceLT,
-    --       UInt8.toUInt32_ofNat, Option.ite_none_left_eq_some, UInt32.not_lt, Option.some.injEq]
-    --     refine ⟨?_, ?_⟩
-    --     · sorry
-    --     · ext
-    --       simp
-    --       sorry
-    --   · sorry
-    -- · simp
-    --   sorry
-    -- · simp
-    --   sorry
-  | case3 => sorry
-  | case4 => sorry
+  match hc : c.utf8Size, c.utf8Size_pos, c.utf8Size_le_four with
+  | 1, _, _ =>
+    have hc' : (String.utf8EncodeChar c).length = 1 := String.length_utf8EncodeChar _ ▸ hc
+    rw [utf8DecodeChar?_append_eq_assemble₁ hc' (parseFirstByte_utf8EncodeChar_eq_done hc)]
+    exact (assemble₁_eq_some_iff_utf8EncodeChar_eq.2 (List.eq_getElem_of_length_eq_one _ hc')).2
+  | 2, _, _ =>
+    have hc' : (String.utf8EncodeChar c).length = 2 := String.length_utf8EncodeChar _ ▸ hc
+    rw [utf8DecodeChar?_append_eq_assemble₂ hc' (parseFirstByte_utf8EncodeChar_eq_oneMore hc)]
+    exact (assemble₂_eq_some_iff_utf8EncodeChar_eq.2 (List.eq_getElem_of_length_eq_two _ hc')).2
+  | 3, _, _ =>
+    have hc' : (String.utf8EncodeChar c).length = 3 := String.length_utf8EncodeChar _ ▸ hc
+    rw [utf8DecodeChar?_append_eq_assemble₃ hc' (parseFirstByte_utf8EncodeChar_eq_twoMore hc)]
+    exact (assemble₃_eq_some_iff_utf8EncodeChar_eq.2 (List.eq_getElem_of_length_eq_three _ hc')).2
+  | 4, _, _ =>
+    have hc' : (String.utf8EncodeChar c).length = 4 := String.length_utf8EncodeChar _ ▸ hc
+    rw [utf8DecodeChar?_append_eq_assemble₄ hc' (parseFirstByte_utf8EncodeChar_eq_threeMore hc)]
+    exact (assemble₄_eq_some_iff_utf8EncodeChar_eq.2 (List.eq_getElem_of_length_eq_four _ hc')).2
 
-theorem String.utf8EncodeChar_eq_singleton {c : Char} (hc : c.val < 128) :
-    String.utf8EncodeChar c = [c.val.toUInt8] := by
-  grind [utf8EncodeChar]
+theorem toByteArray_of_utf8DecodeChar?_eq_some {b : ByteArray} {c : Char} (h : utf8DecodeChar? b 0 = some c) :
+    (String.utf8EncodeChar c).toByteArray = b.extract 0 c.utf8Size := by
+  have := utf8Size_le_of_utf8DecodeChar?_eq_some h
+  match hc : c.utf8Size, c.utf8Size_pos, c.utf8Size_le_four with
+  | 1, _, _ =>
+    have := parseFirstByte_eq_done_of_utf8DecodeChar?_eq_some h hc (by omega)
+    rw [utf8DecodeChar?_eq_assemble₁ (by omega) this] at h
+    rw [ByteArray.extract_add_one (by omega)]
+    congr
+    rw [← assemble₁_eq_some_iff_utf8EncodeChar_eq]
+    exact ⟨this, h⟩
+  | 2, _, _ =>
+    have := parseFirstByte_eq_oneMore_of_utf8DecodeChar?_eq_some h hc (by omega)
+    rw [utf8DecodeChar?_eq_assemble₂ (by omega) this] at h
+    rw [ByteArray.extract_add_two (by omega)]
+    congr
+    rw [← assemble₂_eq_some_iff_utf8EncodeChar_eq]
+    exact ⟨this, h⟩
+  | 3, _, _ =>
+    have := parseFirstByte_eq_twoMore_of_utf8DecodeChar?_eq_some h hc (by omega)
+    rw [utf8DecodeChar?_eq_assemble₃ (by omega) this] at h
+    rw [ByteArray.extract_add_three (by omega)]
+    congr
+    rw [← assemble₃_eq_some_iff_utf8EncodeChar_eq]
+    exact ⟨this, h⟩
+  | 4, _, _ =>
+    have := parseFirstByte_eq_threeMore_of_utf8DecodeChar?_eq_some h hc (by omega)
+    rw [utf8DecodeChar?_eq_assemble₄ (by omega) this] at h
+    rw [ByteArray.extract_add_four (by omega)]
+    congr
+    rw [← assemble₄_eq_some_iff_utf8EncodeChar_eq]
+    exact ⟨this, h⟩
 
-theorem String.utf8EncodeChar_eq_cons_cons {c : Char} (hc₀ : 128 ≤ c.val) (hc₁ : c.val ≤ 0x7ff) :
-    String.utf8EncodeChar c = [(c.val >>>  6).toUInt8 &&& 0x1f ||| 0xc0, c.val.toUInt8 &&& 0x3f ||| 0x80] := by
-  grind [utf8EncodeChar]
-
-theorem String.utf8EncodeChar_eq_cons_cons_cons {c : Char} (hc₀ : 0x7ff < c.val) (hc₁ : c.val ≤ 0xffff) :
-    String.utf8EncodeChar c =
-    [(c.val >>> 12).toUInt8 &&& 0x0f ||| 0xe0,
-     (c.val >>>  6).toUInt8 &&& 0x3f ||| 0x80,
-              c.val.toUInt8 &&& 0x3f ||| 0x80] := by
-  grind [utf8EncodeChar]
-
-theorem String.utf8EncodeChar_eq_cons_cons_cons_cons {c : Char} (hc : 0xffff < c.val) :
-    String.utf8EncodeChar c =
-    [(c.val >>> 18).toUInt8 &&& 0x07 ||| 0xf0,
-     (c.val >>> 12).toUInt8 &&& 0x3f ||| 0x80,
-     (c.val >>>  6).toUInt8 &&& 0x3f ||| 0x80,
-              c.val.toUInt8 &&& 0x3f ||| 0x80] := by
-  grind [utf8EncodeChar]
+/-! # Corollaries -/
 
 theorem eq_of_utf8DecodeChar?_eq_some {b : ByteArray} {c : Char} (h : utf8DecodeChar? b 0 = some c) :
     b = (String.utf8EncodeChar c).toByteArray ++ b.extract c.utf8Size b.size := by
-  conv => lhs; rw [← ByteArray.extract_zero_size (b := b), ByteArray.extract_eq_extract_append_extract (min c.utf8Size b.size) (by simp) (Nat.min_le_right ..)]
-  congr 1
-  · revert h
-    fun_cases utf8DecodeChar? b 0
-    all_goals try (simp; done)
-    all_goals (simp only [Option.some.injEq]); rintro rfl
-    · rename_i hb hp
-      rw [← String.length_utf8EncodeChar, String.utf8EncodeChar_eq_singleton]
-      · simp only [UInt8.toUInt8_toUInt32, List.length_cons, List.length_nil, Nat.zero_add,
-        (by omega : min 1 b.size = 1)]
-        rw [ByteArray.extract_add_one (by omega)]
-      · simp [UInt32.lt_iff_toNat_lt]
-        grind [parseFirstByte, UInt8.lt_iff_toNat_lt]
-    · rename_i _ hp b₀ hb hb₁ b₁ r hr
-      subst b₀ b₁ r
-      rw [← String.length_utf8EncodeChar, String.utf8EncodeChar_eq_cons_cons]
-      · simp [(by omega : min 2 b.size = 2)]
-        rw [ByteArray.extract_add_two (by omega)]
-        congr
-        · sorry
-        · sorry
-      · grind
-      · simp [UInt32.le_iff_toNat_le]
-        · sorry
-    · rename_i _ hp b₀ hb hb₁₂ b₁ b₂ r hr₁ hr₂
-      subst b₀ b₁ b₂ r
-      rw [← String.length_utf8EncodeChar, String.utf8EncodeChar_eq_cons_cons_cons]
-      · simp [(by omega : min 3 b.size = 3)]
-        rw [ByteArray.extract_add_three (by omega)]
-        congr
-        · sorry
-        · sorry
-        · sorry
-      · grind
-      · sorry
-    · rename_i _ hp b₀ hb hb₁₂₃ b₁ b₂ b₃ r hr₁ hr₂
-      subst b₀ b₁ b₂ b₃ r
-      rw [← String.length_utf8EncodeChar, String.utf8EncodeChar_eq_cons_cons_cons_cons]
-      · simp [(by omega : min 4 b.size = 4)]
-        rw [ByteArray.extract_add_four (by omega)]
-        simp [isInvalidContinutationByte_eq_false_iff] at hb₁₂₃
-        congr
-        · sorry
-        · sorry
-        · sorry
-        · sorry
-      · grind
-  · simp only [ByteArray.extract_eq_extract_left, Nat.le_refl, Nat.min_eq_left]
-    omega
+  rw [toByteArray_of_utf8DecodeChar?_eq_some h,
+    ByteArray.extract_append_extract, Nat.zero_min, Nat.max_eq_right (utf8Size_le_of_utf8DecodeChar?_eq_some h),
+    ByteArray.extract_zero_size]
 
 theorem exists_of_utf8DecodeChar?_eq_some {b : ByteArray} {c : Char} (h : utf8DecodeChar? b 0 = some c) :
     ∃ l, b = (String.utf8EncodeChar c).toByteArray ++ l :=
@@ -356,8 +1170,6 @@ theorem utf8DecodeChar?_eq_utf8DecodeChar?_drop {b : ByteArray} {i : Nat} :
       simp [h₄, h₅, h₆, h₇, h₈]
   · rfl
 
-  -- grind
-
 theorem le_size_of_utf8DecodeChar?_eq_some {b : ByteArray} {i : Nat} {c : Char}
     (h : utf8DecodeChar? b i = some c) : i + c.utf8Size ≤ b.size := by
   rw [utf8DecodeChar?_eq_utf8DecodeChar?_drop] at h
@@ -369,5 +1181,8 @@ theorem le_size_of_utf8DecodeChar?_eq_some {b : ByteArray} {i : Nat} {c : Char}
     obtain ⟨h, -⟩ := h
     omega
   omega
+
+def utf8DecodeChar (bytes : ByteArray) (i : Nat) (h : (utf8DecodeChar? bytes i).isSome) : Char :=
+  (utf8DecodeChar? bytes i).get h
 
 end decode
